{"nbformat":4,"nbformat_minor":0,"metadata":{"colab":{"provenance":[],"authorship_tag":"ABX9TyOqGMi7s6/GJ8Q2HMADmsz2"},"kernelspec":{"name":"python3","display_name":"Python 3"},"language_info":{"name":"python"}},"cells":[{"cell_type":"markdown","source":["### Solving Systems of Equations:\n","\n","#### System 1:\n","Given the equations:\n","$$ 3x - 2y = 5 \\quad (1) $$\n","$$ 2x + 3y = 7 \\quad (2) $$\n","\n","**Step 1:** Express \\( x \\) from equation (1):\n","\n","$$ x = \\frac{5 + 2y}{3} $$\n","\n","**Step 2:** Substitute \\( x \\) into equation (2):\n","\n","$$ 2\\left(\\frac{5 + 2y}{3}\\right) + 3y = 7 $$\n","\n","Simplify the equation:\n","\n","$$ \\frac{2(5 + 2y)}{3} + 3y = 7 $$\n","$$ \\frac{10 + 4y}{3} + 3y = 7 $$\n","\n","Multiply by 3 to eliminate the denominator:\n","\n","$$ 10 + 4y + 9y = 21 $$\n","\n","**Step 3:** Solve for \\( y \\):\n","\n","$$ 13y = 11 $$\n","$$ y = \\frac{11}{13} $$\n","\n","**Step 4:** Substitute \\( y = \\frac{11}{13} \\) into the expression for \\( x \\):\n","\n","$$ x = \\frac{5 + 2 \\times \\frac{11}{13}}{3} = \\frac{5 + \\frac{22}{13}}{3} = \\frac{\\frac{65}{13} + \\frac{22}{13}}{3} = \\frac{\\frac{87}{13}}{3} = \\frac{87}{39} = \\frac{29}{13} $$\n","\n","**Solution:** $$ x = \\frac{29}{13}, \\quad y = \\frac{11}{13} $$\n","\n","---\n","\n","#### System 2:\n","Given the equations:\n","$$ 2x - 3y = 10 \\quad (1) $$\n","$$ 4x + 5y = 20 \\quad (2) $$\n","\n","**Step 1:** Multiply equation (1) by 2 to align with the coefficients of \\( x \\) in equation (2):\n","\n","$$ 4x - 6y = 20 \\quad (3) $$\n","\n","**Step 2:** Subtract equation (2) from equation (3):\n","\n","$$ (4x - 6y) - (4x + 5y) = 20 - 20 $$\n","$$ -11y = 0 $$\n","\n","**Step 3:** Solve for \\( y \\):\n","\n","$$ y = 0 $$\n","\n","**Step 4:** Substitute \\( y = 0 \\) into equation (1):\n","\n","$$ 2x - 3(0) = 10 $$\n","$$ 2x = 10 $$\n","$$ x = 5 $$\n","\n","**Solution:** $$ x = 5, \\quad y = 0 $$\n","\n","---\n","\n","#### System 3:\n","Given the equations:\n","$$ 2x - y + z = 3 \\quad (1) $$\n","$$ x + 2y - z = 1 \\quad (2) $$\n","$$ 3x - y + 2z = 11 \\quad (3) $$\n","\n","**Step 1:** Add equation (1) and equation (2) to eliminate \\( z \\):\n","\n","$$\n","(2x - y + z) + (x + 2y - z) = 3 + 1\n","$$\n","This simplifies to:\n","$$\n","3x + y = 4 \\quad (4)\n","$$\n","Now, we have a simpler equation (4) in terms of \\( x \\) and \\( y \\).\n","\n","**Step 2:** Solve equation (4) for \\( y \\):\n","$$\n","y = 4 - 3x \\quad (5)\n","$$\n","\n","**Step 3:** Substitute \\( y = 4 - 3x \\) into equation (2) to eliminate \\( y \\):\n","\n","$$\n","x + 2(4 - 3x) - z = 1\n","$$\n","Simplify:\n","$$\n","x + 8 - 6x - z = 1\n","$$\n","$$\n","-5x + 8 - z = 1\n","$$\n","$$\n","-5x - z = -7\n","$$\n","$$\n","z = 5x + 7 \\quad (6)\n","$$\n","\n","**Step 4:** Substitute \\( y = 4 - 3x \\) and \\( z = 5x + 7 \\) into equation (3):\n","\n","$$\n","3x - (4 - 3x) + 2(5x + 7) = 11\n","$$\n","Simplify:\n","$$\n","3x - 4 + 3x + 10x + 14 = 11\n","$$\n","$$\n","16x + 10 = 11\n","$$\n","$$\n","16x = 1\n","$$\n","$$\n","x = \\frac{1}{16}\n","$$\n","\n","**Step 5:** Substitute \\( x = \\frac{1}{16} \\) into equations (5) and (6) to find \\( y \\) and \\( z \\):\n","\n","For \\( y \\):\n","$$\n","y = 4 - 3 \\times \\frac{1}{16} = 4 - \\frac{3}{16} = \\frac{64}{16} - \\frac{3}{16} = \\frac{61}{16}\n","$$\n","\n","For \\( z \\):\n","$$\n","z = 5 \\times \\frac{1}{16} + 7 = \\frac{5}{16} + \\frac{112}{16} = \\frac{117}{16}\n","$$\n","\n","**Solution for System 3:**\n","$$\n","x = \\frac{1}{16}, \\quad y = \\frac{61}{16}, \\quad z = \\frac{117}{16}\n","$$\n","\n","---\n","\n","#### System 4:\n","Given the equations:\n","$$ 2x - 3y + 4z + 2t = 2 \\quad (1) $$\n","$$ 3x + 2y - 5z + 3t = 3 \\quad (2) $$\n","$$ 4x - 3y + 2z - 5t = 4 \\quad (3) $$\n","$$ 5x + 4y - 3z + 2t = 5 \\quad (4) $$\n","\n","**Step 1:** Add equation (1) and equation (2) to eliminate \\( z \\):\n","\n","$$\n","(2x - 3y + 4z + 2t) + (3x + 2y - 5z + 3t) = 2 + 3\n","$$\n","Simplify:\n","$$\n","5x - y - z + 5t = 5 \\quad (5)\n","$$\n","\n","**Step 2:** Subtract equation (2) from equation (3) to eliminate \\( z \\):\n","\n","$$\n","(4x - 3y + 2z - 5t) - (3x + 2y - 5z + 3t) = 4 - 3\n","$$\n","Simplify:\n","$$\n","x - 5y + 7z - 8t = 1 \\quad (6)\n","$$\n","\n","**Step 3:** Solve equation (5) for \\( z \\):\n","\n","$$\n","z = 5x - y + 5t - 5 \\quad (7)\n","$$\n","\n","**Step 4:** Substitute \\( z \\) from equation (7) into equation (6):\n","\n","$$\n","x - 5y + 7(5x - y + 5t - 5) - 8t = 1\n","$$\n","Simplify:\n","$$\n","x - 5y + 35x - 7y + 35t - 35 - 8t = 1\n","$$\n","$$\n","36x - 12y + 27t = 36 \\quad (8)\n","$$\n","Divide by 3:\n","$$\n","12x - 4y + 9t = 12 \\quad (9)\n","$$\n","\n","**Step 5:** Now, substitute equation (7) into equation (1) and simplify to solve for \\( x, y, t \\).\n"],"metadata":{"id":"LAs0TC0_w2Sb"}},{"cell_type":"code","execution_count":1,"metadata":{"colab":{"base_uri":"https://localhost:8080/"},"id":"BBiBn_U_w1bH","executionInfo":{"status":"ok","timestamp":1729810921989,"user_tz":-120,"elapsed":9650,"user":{"displayName":"Zona CZO","userId":"01264352234259177236"}},"outputId":"f67728bb-4c2f-44d8-df6a-9eae4681dadd"},"outputs":[{"output_type":"stream","name":"stdout","text":["Solution to System 1: {x: 29/13, y: 11/13}\n","Solution to System 2: {x: 5, y: 0}\n","Solution to System 3: {x: -1/4, y: 19/4, z: 33/4}\n","Solution to System 4: {t: 0, x: 1, y: 0, z: 0}\n"]}],"source":["import sympy as sp\n","\n","# System 1\n","x, y = sp.symbols('x y')\n","eq1_1 = sp.Eq(3*x - 2*y, 5)\n","eq1_2 = sp.Eq(2*x + 3*y, 7)\n","sol1 = sp.solve([eq1_1, eq1_2], (x, y))\n","print(f\"Solution to System 1: {sol1}\")\n","\n","# System 2\n","eq2_1 = sp.Eq(2*x - 3*y, 10)\n","eq2_2 = sp.Eq(4*x + 5*y, 20)\n","sol2 = sp.solve([eq2_1, eq2_2], (x, y))\n","print(f\"Solution to System 2: {sol2}\")\n","\n","# System 3\n","z = sp.symbols('z')\n","eq3_1 = sp.Eq(2*x - y + z, 3)\n","eq3_2 = sp.Eq(x + 2*y - z, 1)\n","eq3_3 = sp.Eq(3*x - y + 2*z, 11)\n","sol3 = sp.solve([eq3_1, eq3_2, eq3_3], (x, y, z))\n","print(f\"Solution to System 3: {sol3}\")\n","\n","# System 4\n","z, t = sp.symbols('z t')\n","eq4_1 = sp.Eq(2*x - 3*y + 4*z + 2*t, 2)\n","eq4_2 = sp.Eq(3*x + 2*y - 5*z + 3*t, 3)\n","eq4_3 = sp.Eq(4*x - 3*y + 2*z - 5*t, 4)\n","eq4_4 = sp.Eq(5*x + 4*y - 3*z + 2*t, 5)\n","sol4 = sp.solve([eq4_1, eq4_2, eq4_3, eq4_4], (x, y, z, t))\n","print(f\"Solution to System 4: {sol4}\")\n"]}]}